\documentclass[a4paper]{article}
\usepackage{amsmath}
\usepackage{amsthm}
\usepackage{amsfonts}
\usepackage{amssymb}
\usepackage{bussproofs}
\usepackage{mathtools}
\usepackage{verbatim}
\usepackage{dsfont}
\usepackage[all, 2cell]{xy}
\usepackage[all]{xy}
\newtheorem{theorem}{Theorem}
\newtheorem{lemma}{Lemma}
\newtheorem{defin}{Definition}
\newtheorem{ex}{Example}
\newtheorem{col}{Corollary}
\usepackage{listings} 		% for source code
\date{}
\title{Completeness for modal type theory based on the intuitionistic epistemic logic}

\begin{document}
\maketitle

\begin{defin} Family of relations $\sim_{\alpha, \beta} \subseteq \Lambda_{\textbf{K}} \times \Lambda_{\textbf{K}}$, $\alpha, \beta \in \mathbb{T}_{\textbf{K}}$ is defined by:
\begin{equation}
(x_1, y_1) \sim_{\alpha, \beta} (x_2, y_2) \Leftrightarrow x_i : \alpha \vdash y_i : \beta, i \in \{ 1,2 \} \: \& \: y_2 =_{\beta\eta} y_1 [x_1 := x_2]
\end{equation}
\end{defin}

It is clearly that forall $\alpha, \beta \in \mathbb{T}_{\textbf{K}}$ is an equivalence relation.

Equivalence class for some $\phi, \psi \in \in \mathbb{T}_{\textbf{K}}$ and for some $(M, N)$ such that $M :
\phi \vdash N : \psi$ is defined as:
\begin{equation}
[(M,N)]_{\phi, \psi} = \{ (K, L) | (K, L) \sim_{\phi, \psi} (M, N)\}
\end{equation}

\vspace{\baselineskip}

Let us consider the category $\mathcal{C}_{\lambda}$:
\begin{defin}

$ $

\begin{itemize}
\item $Ob_{\mathcal{C}_{\lambda}} = \{ \mathds{1}\} \cup \{ \hat{\phi} \: | \: \phi \in
\mathbb{T}_{\textbf{K}} \}$
\item $Hom_{\mathcal{C}_{\lambda}}(\hat{\phi},\hat{\psi}) = \{ [(x_1, y_1)]_{\phi, \psi} \: | \: x_1 : \phi
\vdash y_1 : \psi \}$.
\item $[(x_2, y_2)]_{\psi, \tau} \circ [(x_1, y_1)]_{\phi, \psi} = [(x_1, y_2[y_1 := x_2])]_{\phi, \tau}$;
\item $id_{\hat{\phi}} = [(x,x)]_{\phi, \phi}$;
\item $\widehat{\phi \times \psi} = \hat{\phi} \times \hat{\psi}$;
\item $\pi_i = [(x, \pi_i x)]_{\phi_1 \times \phi_2, \phi_i}, i \in \{ 1, 2\}$;
\item $\epsilon = [(x, (\pi_1 x)(\pi_2 x))]_{\phi \rightarrow \psi \times \phi, \psi}$;
\item $\Lambda([(x, M)]_{\phi \times \psi, \tau}) = [(x_1, \lambda x_2. M [x := \langle x_1, x_2
\rangle])]_{\phi, \psi \rightarrow \tau}$.
\end{itemize}
\end{defin}

\begin{defin} Let us functor map $\textbf{K} : \mathcal{C}_{\lambda} \to \mathcal{C}_{\lambda}$, such that:
\begin{itemize}
\item $\textbf{K} : \hat{\phi} \mapsto \hat{\textbf{K}\phi}$;
\item $\textbf{K}(\mathds{1}) = \mathds{1}$
\item $\textbf{K} : [(x_2, y_2)]_{\psi, \tau} \mapsto \textbf{K}([(x_2, y_2)]_{\psi, \tau}) = {K}([(x_2,
y_2)])_{\textbf{K}\psi, \textbf{K}\tau}$;
\item $\textbf{K}([(x_2, y_2)]_{\psi, \tau} \circ [(x_1, y_1)]_{\phi, \psi}) = \textbf{K}([(x_1, y_2[y_1 :=
x_2])])_{\textbf{K}\phi, \textbf{K}\tau}$
\item $\textbf{K} : \hat{\phi} \times \hat{\psi} \mapsto \hat{\textbf{K}\phi} \times \hat{\textbf{K}\psi}$;
\item $\textbf{K} : \hat{\phi} \rightarrow \hat{\psi} \mapsto \hat{\textbf{K}\phi} \rightarrow
\hat{\textbf{K}\psi}$.
\end{itemize}
\end{defin}

\begin{lemma}

$\textbf{K}(\hat{\phi} \times \hat{\psi}) \cong \textbf{K}(\hat{\phi}) \times \textbf{K}(\hat{\psi})$.

\end{lemma}

\begin{proof}

$ $

$\langle \textbf{K}(\pi_1), \textbf{K}(\pi_2) \rangle = \langle \textbf{K}([(x, \pi_1 x)])_{\textbf{K}(\phi \times \psi), \textbf{K}\phi}, \textbf{K}(
[(x, \pi_2 x)])_{\textbf{K}(\phi \times \psi), \textbf{K}\psi} \rangle : \textbf{K}(\hat{\phi} \times
\hat{\psi}) \rightarrow \textbf{K}(\hat{\phi}) \times \textbf{K}(\hat{\psi})$.
\end{proof}

\end{document}
